Changed a condition for interacting modular refinement; new admits generated

src/Syntax.v
@@ -549,6 +549,34 @@ Section GetCalls.
       apply getCallsM_SubList; auto.
   Qed.
 
+  Definition DefCallSub (impl spec: Modules) :=
+    SubList (getDefs spec) (getDefs impl) /\
+    SubList (getCalls spec) (getCalls impl).
+
+  Lemma DefCallSub_refl:
+    forall m, DefCallSub m m.
+  Proof.
+    intros; split; apply SubList_refl.
+  Qed.
+  Hint Immediate DefCallSub_refl.
+
+  Lemma DefCallSub_modular:
+    forall m1 m2 m3 m4,
+      DefCallSub m1 m3 ->
+      DefCallSub m2 m4 ->
+      DefCallSub (ConcatMod m1 m2) (ConcatMod m3 m4).
+  Proof.
+    unfold DefCallSub, SubList; intros; dest; split; intros.
+    - specialize (H e); specialize (H0 e); specialize (H1 e); specialize (H2 e).
+      apply getDefs_in in H3; destruct H3.
+      + apply getDefs_in_1; auto.
+      + apply getDefs_in_2; auto.
+    - specialize (H e); specialize (H0 e); specialize (H1 e); specialize (H2 e).
+      apply getCalls_in in H3; destruct H3.
+      + apply getCalls_in_1; auto.
+      + apply getCalls_in_2; auto.
+  Qed.
+
 End GetCalls.
 
 Section NoInternalCalls.
